src/CoreExpr/Stream.v
@@ -1,5 +1,6 @@
 From Velus Require Import Common.
 From Velus Require Import Operators.
+From Velus Require Import Environment.
 
 From Coq Require Import Setoid.
 From Coq Require Import Morphisms.
@@ -396,6 +397,118 @@ if the clocked stream is [absent] at the corresponding instant. *)
 
   Definition vstr (xss: stream (list const)): stream (list value) :=
     fun n => map (fun c => present (sem_const c)) (xss n).
+
+  (** Restrictions of Environments *)
+  Section HistoryRestriction.
+
+    Definition env := Env.t value.
+    Definition history := Env.t (stream value).
+
+    Definition restr_hist (H : history) (n: nat): env :=
+      Env.map (fun xs => xs n) H.
+
+    Lemma Env_find_restr_hist:
+      forall H x i,
+        Env.find x (restr_hist H i) = option_map (fun xs => xs i) (Env.find x H).
+    Proof.
+      unfold restr_hist. now setoid_rewrite Env.Props.P.F.map_o.
+    Qed.
+
+    Lemma Env_add_restr_hist:
+      forall H x s i,
+        Env.Equal (restr_hist (Env.add x s H) i) (Env.add x (s i) (restr_hist H i)).
+    Proof.
+      intros H x s i x'. unfold restr_hist.
+      setoid_rewrite Env.Props.P.F.map_o.
+      destruct (ident_eq_dec x' x).
+      - subst. now setoid_rewrite Env.gss.
+      - now setoid_rewrite Env.gso; auto; rewrite <-Env.Props.P.F.map_o.
+    Qed.
+
+    Lemma Env_In_restr_hist:
+      forall H x i,
+        Env.In x H <-> Env.In x (restr_hist H i).
+    Proof.
+      intros. unfold restr_hist.
+      now rewrite Env.Props.P.F.map_in_iff.
+    Qed.
+
+    Lemma Env_dom_restr_hist:
+      forall H xs i,
+        Env.dom H xs <-> Env.dom (restr_hist H i) xs.
+    Proof.
+      split; intros HH; apply Env.dom_intro; intro x;
+        apply Env.dom_use with (x0:=x) in HH;
+        now rewrite <-HH, Env_In_restr_hist.
+    Qed.
+
+    Lemma stream_env_to_env_stream:
+      forall xs (H : stream (Env.t value)),
+        (forall i, Env.dom (H i) xs) ->
+        (exists (H' : Env.t (stream value)),
+            (forall i, Env.Equal (H i) (restr_hist H' i))
+            /\ (forall x, In x xs -> Env.find x H' = Some (fun i => match Env.find x (H i) with
+                                                            Some v => v | None => absent end))).
+    Proof.
+      setoid_rewrite <-(nub_same_elements ident_eq_dec).
+      intros ys.
+      pose proof (NoDup_nub ident_eq_dec ys) as NDN; revert NDN.
+      induction (nub ident_eq_dec ys) as [|x xs IH]; clear ys;
+        intros ND H DH.
+      - (* environment is empty *)
+        exists (Env.empty _). split; [|now inversion 1].
+        intros i y. specialize (DH i).
+        apply Env.dom_use with (x:=y) in DH.
+        unfold Env.from_list. rewrite Env_find_restr_hist, Env.gempty; simpl.
+        apply Env.Props.P.F.not_find_in_iff; rewrite DH; auto.
+      - (* environment is not empty *)
+        inversion ND as [|? ? Nx ND']; subst.
+        exists (Env.add x (fun i => match Env.find x (H i) with Some y => y | None => absent end)
+                   (Env.from_list (map (fun x => (x,
+                                               fun i => match Env.find x (H i) with Some y => y | None => absent end)) xs))).
+        setoid_rewrite Env_add_restr_hist.
+        split.
+        + (* show point-wise equality of H and H' *)
+          intro i.
+          assert (forall i, Env.In x (H i)) as Ix
+              by (intro j; specialize (DH j);
+                  apply Env.dom_use with (x0:=x) in DH; firstorder).
+          setoid_rewrite Env.In_find in Ix.
+          destruct (Ix i) as (v & Ixi). rewrite Ixi.
+          apply Env.add_remove in Ixi. rewrite Ixi at 1.
+          apply Env.Equal_add_both.
+          assert (forall i, Env.dom (Env.remove x (H i)) xs) as Dr.
+          { intro j. specialize (DH j).
+            apply Env.dom_cons_remove with (x0:=x) in DH. simpl in DH.
+            rewrite nequiv_decb_refl, not_in_filter_nequiv_decb in DH; auto. }
+          specialize (IH ND' (fun i => Env.remove x (H i)) Dr) as (H' & IH1 & IH2).
+          intro y. destruct (in_dec ident_eq_dec y xs) as [Iy|Ny].
+          * (* element in domain of environment *)
+            rewrite IH1.
+            assert (y <> x) by (intro; subst; auto).
+            repeat rewrite Env_find_restr_hist. rewrite IH2; auto; clear IH2.
+            simpl. specialize (Dr i). apply Env.dom_use with (x0:=y) in Dr.
+            destruct Dr as (Dr1 & Dr2). specialize (Dr2 Iy).
+            rewrite Env.In_find in Dr2. destruct Dr2 as (yv & Fy); rewrite Fy.
+            erewrite Env.find_In_from_list.
+            2:now apply in_map_iff; eauto.
+            now simpl; rewrite Env.gro in Fy; auto; rewrite Fy.
+            now apply fst_NoDupMembers; rewrite map_map, map_id.
+          * (* element outside domain of environment *)
+            rewrite Env.find_not_In_dom with (1:=Dr i) (2:=Ny).
+            rewrite Env.find_not_In_dom with (2:=Ny); auto.
+            apply Env_dom_restr_hist, Env.dom_from_list_map_fst;
+              [apply fst_NoDupMembers|]; now rewrite map_map, map_id.
+        + (* show characterization of H' *)
+          intros y Iy. inv Iy. now rewrite Env.gss.
+          rewrite Env.gso; [|intro; subst; auto].
+          erewrite Env.find_In_from_list. reflexivity.
+          now apply in_map_iff; eauto.
+          apply fst_NoDupMembers. rewrite map_map; simpl.
+          rewrite map_id. inv ND; auto.
+    Qed.
+
+  End HistoryRestriction.
 
 End STREAM.
 
